thinking about iteration

ordered_map.dfy
@@ -5,23 +5,22 @@ abstract module Ordered_Map refines Map {
   import Key_Space : Total_Order
   type Key = Key_Space.Element
 
-  datatype OrderedQueryResult = NoMoreElements | OrderedQueryResult(key: Key)
+  // Return a map containing just the entries with keys in the interval [begin, end].
+  // If you don't want begin or end in the result, just Undefine them from the result.
+  method Subrange(m: Map, begin: Key, end: Key) returns (submap: Map)
+    ensures Interpretation(submap).Keys ==
+      set k | k in Interpretation(m).Keys && Key_Space.lte(begin, k) && Key_Space.lte(k, end);
+    ensures forall k :: k in Interpretation(submap) ==> Interpretation(submap)[k] == Interpretation(m)[k];
     
-  method Successor(m: Map, key: Key) returns (result: OrderedQueryResult)
-    ensures result.NoMoreElements?
-      ==> (forall k :: k in Interpretation(m) ==> Key_Space.lte(k, key));
-    ensures result.OrderedQueryResult?
-      ==> (result.key in Interpretation(m) &&
-           Key_Space.lt(key, result.key) &&
-           (forall k :: Key_Space.lt(key, k) && Key_Space.lt(k, result.key) ==> k !in Interpretation(m)));
+  method FirstKey(m: Map) returns (key: Key)
+    requires !IsEmpty(m);
+    ensures key in Interpretation(m);
+    ensures forall k :: k in Interpretation(m) ==> Key_Space.lte(key, k);
 
-  method Predecessor(m: Map, key: Key) returns (result: OrderedQueryResult)
-    ensures result.NoMoreElements?
-      ==> (forall k :: k in Interpretation(m) ==> Key_Space.lte(key, k));
-    ensures result.OrderedQueryResult?
-      ==> (result.key in Interpretation(m) &&
-           Key_Space.lt(result.key, key) &&
-           (forall k :: Key_Space.lt(result.key, k) && Key_Space.lt(k, key) ==> k !in Interpretation(m)));
+  method LastKey(m: Map) returns (key: Key)
+    requires !IsEmpty(m);
+    ensures key in Interpretation(m);
+    ensures forall k :: k in Interpretation(m) ==> Key_Space.lte(k, key);
 }
 
 // Here's a model of the above abstraction, just to show it can be done.
@@ -31,9 +30,15 @@ abstract module Sorted_Sequence_Map refines Ordered_Map {
 
   function method {:opaque} Interpretation(m: Map) : map<Key, Value>
     ensures forall k :: k in Interpretation(m) <==> exists i :: 0 <= i < |m| && k == m[i].key;
+    ensures forall i :: 0 <= i < |m| ==> Interpretation(m)[m[i].key] == m[i].value;
+    ensures Interpretation(m) == map[] <==> m == [];
   {
     if |m| == 0 then map[]
-    else Interpretation(m[1..])[m[0].key := m[0].value]
+    else
+      var s := Interpretation(m[1..]);
+      assert forall i :: 0 < i < |m| ==> Key_Space.lt(m[0].key, m[i].key); // Observe
+      var t := s[m[0].key := m[0].value];
+      t
   }
 
   method EmptyMap() returns (empty_map: Map) {
@@ -69,8 +74,21 @@ abstract module Sorted_Sequence_Map refines Ordered_Map {
     }
   }
 
+  method Defines(m: Map, key: Key) returns (result: bool) {
+    if |m| == 0 {
+      result := false;
+    } else if key == m[0].key {
+      result := true;
+    } else {
+      result := Defines(m[1..], key);
+    }
+  }
+  
+  predicate method IsEmpty(m: Map) {
+    m == []
+  }
+  
   method Query(m: Map, key: Key) returns (result: QueryResult) {
-    reveal_Interpretation();
     if |m| == 0 {
       result := DNE;
     } else if key == m[0].key {
@@ -80,31 +98,63 @@ abstract module Sorted_Sequence_Map refines Ordered_Map {
     }
   }
 
-  method Successor(m: Map, key: Key) returns (result: OrderedQueryResult) {
-    if |m| == 0 {
-      result := NoMoreElements;
-    } else if Key_Space.lt(key, m[0].key) {
-      assert forall i :: 0 < i < |m| ==> Key_Space.lt(m[0].key, m[i].key); // Observe
-      result := OrderedQueryResult(m[0].key);
-    } else {
-      result := Successor(m[1..], key);
-    }
+  method Evaluate(m: Map, key: Key) returns (value: Value) {
+    var t := Query(m, key);
+    value := t.value;
   }
 
-  method Predecessor(m: Map, key: Key) returns (result: OrderedQueryResult) {
+  method Subrange(m: Map, begin: Key, end: Key) returns (submap: Map) {
+    reveal_Interpretation();
     if |m| == 0 {
-      result := NoMoreElements;
-    } else if Key_Space.lt(m[|m|-1].key, key) {
+      submap := m;
+    } else if Key_Space.lt(m[0].key, begin) {
+      submap := Subrange(m[1..], begin, end);
+    } else if Key_Space.lt(end, m[|m|-1].key) {
       assert forall i :: 0 <= i < |m|-1 ==> Key_Space.lt(m[i].key, m[|m|-1].key); // Observe
-      result := OrderedQueryResult(m[|m|-1].key);
+      submap := Subrange(m[..|m|-1], begin, end);
     } else {
-      result := Predecessor(m[..|m|-1], key);
+      assert forall i :: 0 < i < |m| ==> Key_Space.lt(m[0].key, m[i].key); // Observe
+      assert forall i :: 0 <= i < |m|-1 ==> Key_Space.lt(m[i].key, m[|m|-1].key); // Observe
+      submap := m;
     }
   }
+  
+  method AKey(m: Map) returns (key: Key) {
+    key := m[0].key;
+  }
+
+  method FirstKey(m: Map) returns (key: Key) {
+    assert forall i :: 0 < i < |m| ==> Key_Space.lt(m[0].key, m[i].key); // Observe
+    key := m[0].key;
+  }
+
+  method LastKey(m: Map) returns (key: Key) {
+    assert forall i :: 0 <= i < |m|-1 ==> Key_Space.lt(m[i].key, m[|m|-1].key); // Observe
+    key := m[|m|-1].key;
+  }
+
 }
 
 // Example instantiation
 module Sorted_Sequence_Integer_Integer_Map refines Sorted_Sequence_Map {
   import Key_Space = Integer_Order
   type Value = int
+}
+
+method Main() {
+  var m := Sorted_Sequence_Integer_Integer_Map.EmptyMap();
+  m := Sorted_Sequence_Integer_Integer_Map.Define(m, 7, 49);
+  m := Sorted_Sequence_Integer_Integer_Map.Define(m, 3, 9);
+  m := Sorted_Sequence_Integer_Integer_Map.Define(m, 12, 144);
+  m := Sorted_Sequence_Integer_Integer_Map.Define(m, -6, 36);
+
+  var iter := Sorted_Sequence_Integer_Integer_Map.Subrange(m, 0, 12);
+  while !Sorted_Sequence_Integer_Integer_Map.IsEmpty(iter)
+    decreases |Sorted_Sequence_Integer_Integer_Map.Interpretation(iter).Keys|
+  {
+    var k := Sorted_Sequence_Integer_Integer_Map.FirstKey(iter);
+    var v := Sorted_Sequence_Integer_Integer_Map.Evaluate(iter, k);
+    print k, " ", v, "\n";
+    iter := Sorted_Sequence_Integer_Integer_Map.Undefine(iter, k);
+  }
 }
