map.dfy
@@ -1,0 +1,249 @@
+// A Map that you can query, but you can't insert/remove elements
+// Iterators will be read-only maps from int -> kvpair
+// This abstract module doesn't define a constructor, since the
+// input to construct a Readonly_Map will naturally be
+// implementation-specific.
+abstract module Readonly_Map {
+  type Key(!new,==)
+  type Value
+  type Map
+
+  datatype Query_Result = DNE | Query_Result(value: Value)
+
+  function Interpretation(m: Map) : map<Key, Value>
+
+  method Is_Empty(m: Map) returns (result: bool)
+    ensures result <==> Interpretation(m) == map[];
+
+  method Defines(m: Map, key: Key) returns (result: bool)
+    ensures result == (key in Interpretation(m));
+      
+  method Query(m: Map, key: Key) returns (result: Query_Result)
+    ensures key in Interpretation(m) ==> result == Query_Result(Interpretation(m)[key]);
+    ensures key !in Interpretation(m) ==> result == DNE;
+
+  method Evaluate(m: Map, key: Key) returns (value: Value)
+    requires key in Interpretation(m);
+    ensures value == Interpretation(m)[key];
+}
+
+// Just add methods for creating modified versions of the given Map
+abstract module Map refines Readonly_Map {
+
+  method Empty_Map() returns (empty_map: Map)
+    ensures Interpretation(empty_map) == map[];
+    
+  method Define(m: Map, key: Key, value: Value) returns (new_map: Map)
+    ensures Interpretation(new_map) == Interpretation(m)[key := value];
+
+  method Undefine(m: Map, key: Key) returns (new_map: Map)
+    ensures Interpretation(new_map).Keys == Interpretation(m).Keys - {key};
+    ensures forall key' :: key' in Interpretation(new_map)
+      ==> Interpretation(new_map)[key'] == Interpretation(m)[key'];
+}
+
+// An iterator is a Readonly_Map from [0, 1, ...] to kvpairs of its underlying map
+abstract module Iterator refines Readonly_Map {
+  import Underlying_Map : Readonly_Map
+  datatype KVPair = KVPair(key: Underlying_Map.Key, value: Underlying_Map.Value)
+
+  type Key = int
+  type Value = KVPair
+  type Iterator = Map
+
+  method Construct(m: Underlying_Map.Map) returns (iter: Iterator)
+    ensures forall i :: i in Interpretation(iter).Keys <==> 0 <= i < |Underlying_Map.Interpretation(m)|;
+    ensures forall k, v :: k in Underlying_Map.Interpretation(m) && Underlying_Map.Interpretation(m)[k] == v ==>
+            exists i :: i in Interpretation(iter).Keys && Interpretation(iter)[i] == KVPair(k, v);
+}
+
+
+// Let's see if we can build one of these mofos from the builtin map
+
+abstract module Builtin_Map refines Map {
+  type Map = map<Key, Value>
+
+  function Interpretation(m: Map) : map<Key, Value> {
+    m
+  }
+
+  method Is_Empty(m: Map) returns (result: bool) {
+    result := |m| == 0;
+  }
+
+  method Defines(m: Map, key: Key) returns (result: bool) {
+    result := key in m;
+  }
+
+  method Query(m: Map, key: Key) returns (result: Query_Result) {
+    if key in m {
+      result := Query_Result(m[key]);
+    } else {
+      result := DNE;
+    }
+  }
+
+  method Evaluate(m: Map, key: Key) returns (value: Value) {
+    value := m[key];
+  }
+
+  method Empty_Map() returns (empty_map: Map) {
+    empty_map := map[];
+  }
+
+  method Define(m: Map, key: Key, value: Value) returns (new_map: Map) {
+    new_map := m[key := value];
+  }
+
+  method Undefine(m: Map, key: Key) returns (new_map: Map) {
+    new_map := map k | k in m.Keys && k != key :: m[k];
+  }
+
+}
+
+abstract module Builtin_Map_Sequence_Iterator refines Iterator {
+  import Underlying_Map = Builtin_Map
+  type Map = seq<KVPair>
+
+  function Interpretation(m: Map) : map<Key, Value> {
+    map i: int | 0 <= i < |m| :: m[i]
+  }
+
+  method Is_Empty(m: Map) returns (result: bool) {
+    assert |m| > 0 ==> 0 in Interpretation(m).Keys; // Observe
+    result := |m| == 0;
+  }
+
+  method Defines(m: Map, key: Key) returns (result: bool) {
+    result := 0 <= key < |m|;
+  }
+
+  method Query(m: Map, key: Key) returns (result: Query_Result) {
+    if 0 <= key < |m| {
+      result := Query_Result(m[key]);
+    } else {
+      result := DNE;
+    }
+  }
+
+  method Evaluate(m: Map, key: Key) returns (value: Value) {
+    value := m[key];
+  }
+
+  function method id(x: int) : int
+  { x }
+  
+  method Construct(m: Underlying_Map.Map) returns (iter: Iterator)
+    ensures |iter| == |m|;
+    // ensures forall k, v :: k in m && m[k] == v ==> exists i :: 0 <= i < |iter| && iter[i] == KVPair(k, v);
+  {
+    if |m| == 0 {
+      iter := [];
+    } else {
+      var key :| key in m;
+      var value := m[key];
+      var m_without_key := map x | x in m && x != key :: m[x];
+      var tail := Construct(m_without_key);
+      iter := tail + [KVPair(key, value)];
+
+      forall k | k in Underlying_Map.Interpretation(m)
+        ensures forall k, v :: k in Underlying_Map.Interpretation(m) && Underlying_Map.Interpretation(m)[k] == v ==>
+        exists i :: i in Interpretation(iter).Keys && Interpretation(iter)[i] == KVPair(k, v);
+
+      {
+        var v := Underlying_Map.Interpretation(m);
+      }
+      
+      // assert m == Underlying_Map.Interpretation(m);
+      //assert forall i :: i in Interpretation(iter).Keys <==> 0 <= i < |iter|;
+      // assert forall i :: i in Interpretation(iter) ==> Interpretation(iter)[i] == iter[i];
+      
+      // assert Interpretation(iter) == Interpretation(tail)[|tail| := KVPair(k, v)];
+      // assert |tail| !in Interpretation(tail);
+      // assert iter[|iter|-1] == KVPair(k, v);
+      
+      assert m_without_key.Keys == m.Keys - {key}; // Observe?
+      assert |m_without_key.Keys| == |m.Keys|-1; // Observe?
+    }
+  }
+}
+
+
+
+
+
+
+
+
+
+
+
+
+
+
+
+
+// abstract module Mutable_Map {
+
+//   type Key(==)
+//   type Value
+
+//   datatype QueryResult = DNE | QueryResult(Value)
+  
+//   trait Map {
+//     function method Interpretation() : map<Key, Value>
+//       reads this;
+
+//     method Define(key: Key, value: Value)
+//       ensures Interpretation() == old(this.Interpretation())[key := value];
+//       modifies this;
+        
+//     method Undefine(key: Key)
+//       ensures Interpretation().Keys == old(this.Interpretation().Keys) - {key};
+//       ensures forall key' :: key' in Interpretation() ==> Interpretation()[key'] == old(this.Interpretation())[key'];
+//       modifies this;
+          
+//      method Query(key: Key)
+//       returns (result: QueryResult)
+//       ensures key in Interpretation() ==> result == QueryResult(Interpretation()[key]);
+//       ensures key !in Interpretation() ==> result == DNE;
+//   }
+
+//   class BuiltinMap extends Map {
+//     var contents: map<Key, Value>
+
+//     function method Interpretation() : map<Key, Value>
+//       reads this;
+//     {
+//       contents
+//     }
+
+//     method Define(key: Key, value: Value)
+//       ensures Interpretation() == old(this.Interpretation())[key := value];
+//       modifies this;
+//     {
+//       contents := contents[key := value];
+//     }
+    
+//     method Undefine(key: Key)
+//       ensures Interpretation().Keys == old(this.Interpretation().Keys) - {key};
+//       ensures forall key' :: key' in Interpretation() ==> Interpretation()[key'] == old(this.Interpretation())[key'];
+//       modifies this;
+//     {
+//       contents := map key' : Key | key' in contents && key' != key :: contents[key'];
+//     }
+
+//     // I don't know why this won't compile.  Seems like a dafny bug to me...
+//     method Query(key: Key)
+//       returns (result: QueryResult)
+//       ensures key in Interpretation() ==> result == QueryResult(Interpretation()[key]);
+//       ensures key !in Interpretation() ==> result == DNE;
+//     {
+//       if key in contents {
+//         result := QueryResult(contents[key]);
+//       } else {
+//         result := DNE;
+//       }
+//     }
+//   }
+// }
